just use semireducible in both places

src/Init/Data/Fin/Fold.lean
@@ -16,14 +16,14 @@ namespace Fin
   @[semireducible] loop (x : α) (i : Nat) : α :=
     if h : i < n then loop (f x ⟨i, h⟩) (i+1) else x
   termination_by n - i
+  decreasing_by decreasing_trivial_pre_omega
 
 /-- Folds over `Fin n` from the right: `foldr 3 f x = f 0 (f 1 (f 2 x))`. -/
-@[inline] def foldr (n) (f : Fin n → α → α) (init : α) : α := loop n (Nat.le_refl n) init where
+@[inline] def foldr (n) (f : Fin n → α → α) (init : α) : α := loop ⟨n, Nat.le_refl n⟩ init where
   /-- Inner loop for `Fin.foldr`. `Fin.foldr.loop n f i x = f 0 (f ... (f (i-1) x))`  -/
-  loop : (i : _) → i ≤ n → α → α
-  | 0, _, x => x
-  | i+1, h, x => loop i (Nat.le_of_lt h) (f ⟨i, h⟩ x)
-  termination_by structural i => i
+  @[semireducible] loop : {i // i ≤ n} → α → α
+  | ⟨0, _⟩, x => x
+  | ⟨i+1, h⟩, x => loop ⟨i, Nat.le_of_lt h⟩ (f ⟨i, h⟩ x)
 
 /--
 Folds a monadic function over `Fin n` from left to right:
@@ -176,19 +176,17 @@ theorem foldl_eq_foldlM (f : α → Fin n → α) (x) :
 /-! ### foldr -/
 
 theorem foldr_loop_zero (f : Fin n → α → α) (x) :
-    foldr.loop n f 0 (Nat.zero_le _) x = x := by
+    foldr.loop n f ⟨0, Nat.zero_le _⟩ x = x := by
   rw [foldr.loop]
 
 theorem foldr_loop_succ (f : Fin n → α → α) (x) (h : i < n) :
-    foldr.loop n f (i+1) h x = foldr.loop n f i (Nat.le_of_lt h) (f ⟨i, h⟩ x) := by
+    foldr.loop n f ⟨i+1, h⟩ x = foldr.loop n f ⟨i, Nat.le_of_lt h⟩ (f ⟨i, h⟩ x) := by
   rw [foldr.loop]
 
 theorem foldr_loop (f : Fin (n+1) → α → α) (x) (h : i+1 ≤ n+1) :
-    foldr.loop (n+1) f (i+1) h x =
-      f 0 (foldr.loop n (fun j => f j.succ) i (Nat.le_of_succ_le_succ h) x) := by
-  induction i generalizing x with
-  | zero => simp [foldr_loop_succ, foldr_loop_zero]
-  | succ i ih => rw [foldr_loop_succ, ih]; rfl
+    foldr.loop (n+1) f ⟨i+1, h⟩ x =
+      f 0 (foldr.loop n (fun j => f j.succ) ⟨i, Nat.le_of_succ_le_succ h⟩ x) := by
+  induction i generalizing x <;> simp [foldr_loop_zero, foldr_loop_succ, *]
 
 @[simp] theorem foldr_zero (f : Fin 0 → α → α) (x) : foldr 0 f x = x :=
   foldr_loop_zero ..
